eve/Src/framework/eiffel2boogie/tests/framing/ownership/observer_one_to_many/f_oom_subject_d.e
@@ -34,25 +34,23 @@ feature
 			is_wrapped -- default: public
 			across observers as o all o.item.is_wrapped end -- default: public
 
-			modify_field ("value", Current)
-			modify_field ("cache", observers_list.sequence)
+			modify_field (["value", "closed"], Current)
+			modify_field (["cache", "closed"], observers_list.sequence)
 		local
 			i: INTEGER
-			l_old_sequence: MML_SET [F_OOM_OBSERVER_D]
 		do
 			unwrap -- default: public
 			unwrap_all (observers)
-			check across observers as o all o.item.inv end end
 
 			value := new_val
-			check across observers as o all o.item.inv_without ("cache_synchronized") end end
 			from
 				i := 1
 			invariant
---				across 1 |..| (i - 1) as j all observers_list[j.item].cache = new_val end				
-				attached {F_OOM_LIST [F_OOM_OBSERVER_D]} observers_list
-				across observers_list.sequence as o all attached {F_OOM_OBSERVER_D} o.item end
-				across observers as o all o.item.is_open and o.item.inv_without ("cache_synchronized") end
+				across observers_list.sequence as o all
+					o.item.is_open and o.item.inv_without ("cache_synchronized")
+				end
+				is_open and inv
+				value = new_val
 			until
 				i > observers_list.count
 			loop
