eve/Src/framework/eiffel2boogie/translation/e2b_name_translator.e
@@ -79,22 +79,6 @@ feature -- Access
 			result_attached: attached Result
 		end
 
-	boogie_name_for_field_preservation_function (a_feature: FEATURE_I; a_context_type: TYPE_A): STRING
-			-- Name for feature `a_feature'.
-		require
-			a_feature_attached: attached a_feature
-			a_context_type_attached: attached a_context_type
-		local
-			l_type_name: STRING
-			l_feature_name: STRING
-		do
-			l_type_name := boogie_name_for_type (a_context_type)
-			l_feature_name := a_feature.feature_name_32.as_lower
-			Result := "preserves." + l_type_name + "." + l_feature_name
-		ensure
-			result_attached: attached Result
-		end
-
 	boogie_name_for_invariant_function (a_type: TYPE_A): STRING
 			-- Name invariant function of `a_type'.
 		require
